@prefix : <https://joinup.ec.europa.eu/collection/elis/1.0.0/refdata/cissv-ap#> .
@prefix dc: <http://purl.org/dc/elements/1.1/> .
@prefix owl: <http://www.w3.org/2002/07/owl#> .
@prefix rdf: <http://www.w3.org/1999/02/22-rdf-syntax-ns#> .
@prefix xml: <http://www.w3.org/XML/1998/namespace> .
@prefix xsd: <http://www.w3.org/2001/XMLSchema#> .
@prefix rdfs: <http://www.w3.org/2000/01/rdf-schema#> .
@prefix skos: <http://www.w3.org/2004/02/skos/core#> .
@prefix dcterms: <http://purl.org/dc/terms/> .
@base <https://joinup.ec.europa.eu/collection/elis/1.0.0/refdata/cissv-ap#> .

<https://joinup.ec.europa.eu/collection/elis/1.0.0/refdata/eiraviews#> rdf:type owl:Ontology ;
                                                                                 owl:versionIRI <https://joinup.ec.europa.eu/collection/elis/1.0.0/refdata/cissv-ap#> .

#################################################################
#    Individuals
#################################################################

:CISSV-AP rdf:type owl:NamedIndividual ,
                            skos:ConceptScheme ;
                            skos:prefLabel "Core Interoperability Standards and Specifications Vocabulary" ;
                            skos:definition "The entities defining the main concepts needed to configure a set of interoperability specification profiles."@en .

:InteroperabilitySpecification rdf:type owl:NamedIndividual ,
                            skos:Concept ;
                            skos:prefLabel "Interoperability Specification" ;
                            skos:definition "An Interoperability Specification is a document containing agreed normative statements for Solution Building Blocks used in an information exchange context. It can refer to existing standards or specifications (EIRA)."@en ;
                            skos:inScheme :CISSV-AP .

:InteroperabilitySpecificationDomain rdf:type owl:NamedIndividual ,
                            skos:Concept ;
                            skos:prefLabel "Interoperability Specification Domain" ;
                            skos:definition "Use case of a set of interoperability specifications. Domains in EIRA CISSV-AP will be in a business agnostic context and they are a design decision."@en ;
                            skos:inScheme :CISSV-AP .                
                            
:InteroperabilitySpecificationConfiguration rdf:type owl:NamedIndividual ,
                            skos:Concept ;
                            skos:prefLabel "Interoperability Specification Configuration" ;
                            skos:definition "Set of Interoperability Application Profiles of an Interoperability Specification."@en ;
                            skos:inScheme :CISSV-AP .

:InteroperabilitySpecificationConfigurationComponent rdf:type owl:NamedIndividual ,
                            skos:Concept ;
                            skos:prefLabel "Interoperability Specification Configuration Component" ;
                            skos:definition "Element that is part of an Interoperability Specification Configuration."@en ;
                            skos:inScheme :CISSV-AP . 

:InteroperabilityApplicationProfile rdf:type owl:NamedIndividual ,
                            skos:Concept ;
                            skos:prefLabel "Interoperability Application Profile" ;
                            skos:definition "Extension and customization of a standard for its implementation together with other standards."@en ;
                            skos:inScheme :CISSV-AP .
                            
:Standard rdf:type owl:NamedIndividual ,
                            skos:Concept ;
                            skos:prefLabel "Standard" ;
                            skos:definition "Document that provides requirements, specifications, guidelines or characteristics that can be used consistently to ensure that materials, products, processes and services are fit for their purpose (ISO)."@en ;
                            skos:inScheme :CISSV-AP .                              
                                                              
